progress on ed25519 implem

code/experimental/ed25519/Hacl.Impl.Ed25519.Sign.fst
@@ -2,3 +2,15 @@ module Hacl.Impl.Ed25519.Sign
 
 open FStar.Buffer
 
+let hint8_p = buffer Hacl.UInt8.t
+
+val sign:
+  signature:hint8_p{length signature = 64} ->
+  secret:hint8_p{length secret = 32} ->
+  msg:hint8_p ->
+  len:UInt32.t{UInt32.v len = length msg} ->
+  Stack unit
+    (requires (fun h -> live h signature /\ live h msg /\ live h secret))
+    (ensures (fun h0_ h1 -> live h0 secret /\ live h0 secret /\ live h1 signature /\ modifies_1 signature h0 h1))
+let sign signature secret msg len =
+  
