code/experimental/ed25519/Hacl.Impl.Ed25519.PointCompress.fst
@@ -1,0 +1,30 @@
+module Hacl.Impl.Ed25519.PointCompress
+
+open FStar.Buffer
+open Hacl.UInt64
+open Hacl.Bignum25519
+
+
+let hint64_p = buffer t
+
+val point_compress:
+  out:hint64_p{length out = 5} ->
+  p:Hacl.Impl.Ed25519.ExtPoint.point ->
+  Stack unit
+    (requires (fun h -> live h out /\ live h p))
+    (ensures (fun h0 _ h1 -> live h1 out /\ live h0 p /\ modifies_1 out h0 h1))
+let point_compress out p =
+  push_frame();
+  let tmp  = create (Hacl.Cast.uint64_to_sint64 0uL) 10ul in
+  let zinv = Buffer.sub tmp 0ul 5ul in
+  let x    = Buffer.sub tmp 5ul 5ul in
+  let px   = Hacl.Impl.Ed25519.ExtPoint.getx p in
+  let py   = Hacl.Impl.Ed25519.ExtPoint.gety p in
+  let pz   = Hacl.Impl.Ed25519.ExtPoint.getz p in
+  Hacl.Bignum25519.inverse zinv pz;
+  Hacl.Bignum25519.fmul x   px zinv;
+  Hacl.Bignum25519.fmul out py zinv;
+  let b = x.(0ul) &^ 1uL in
+  let out4 = out.(4ul) in
+  out.(4ul) <- out4 +^ (b <<^ 51ul);
+  pop_frame()
