code/experimental/ed25519/Hacl.Impl.Ed25519.SecretExpand.fst
@@ -1,0 +1,20 @@
+module Hacl.Impl.Ed25519.SecretExpand
+
+open FStar.Buffer
+open Hacl.UInt8
+
+let hint8_p = buffer t
+
+val secret_expand:
+  expanded:hint8_p{length expanded = 64} ->
+  secret:hint8_p{length secret = 32} ->
+  Stack unit
+    (requires (fun h -> live h expanded /\ live h secret))
+    (ensures (fun h0 _ h1 -> live h1 expanded /\ live h0 secret /\ modifies_1 expanded h0 h1))
+let secret_expand expanded secret =
+  Hacl.Impl.Sha512.sha512 expanded secret 32ul;
+  let h_low = Buffer.sub expanded 0ul 32ul in
+  let h_low0  = h_low.( 0ul) in
+  let h_low31 = h_low.(31ul) in
+  h_low.( 0ul) <- (h_low0 &^ 0xf8uy);
+  h_low.(31ul) <- ((h_low31 &^ 127uy) |^ 64uy)
